DataflowRewriter/Rewrites/MuxTaggedRewriteCorrect.lean
@@ -120,190 +120,188 @@ def rhsModuleType (Tag T : Type _) : Type := by
 
 attribute [dmod] Batteries.AssocList.find? BEq.beq
 
-instance {Tag T} : MatchInterface (rhsModule Tag T) (lhs_intModule Tag T) where
-  input_types := by
-    intro ident;
-    by_cases h : (Batteries.AssocList.contains ↑ident (rhsModule Tag T).inputs)
-    · have h' := AssocList.keysInMap h; fin_cases h' <;> rfl
-    · have h' := AssocList.keysNotInMap h; dsimp [drunfold, AssocList.keysList] at h' ⊢
-      simp at h'; let ⟨ ha, hb, hc ⟩ := h'; clear h'
-      simp only [Batteries.AssocList.find?_eq, Batteries.AssocList.toList]
-      rcases ident with ⟨ i1, i2 ⟩;
-      repeat (rw [List.find?_cons_of_neg]; rotate_left; simp; intros; subst_vars; solve_by_elim)
-      sorry
-  output_types := by
-    intro ident;
-    by_cases h : (Batteries.AssocList.contains ↑ident (rhsModule Tag T).outputs)
-    · have h' := AssocList.keysInMap h; fin_cases h' <;> rfl
-    · have h' := AssocList.keysNotInMap h; dsimp [drunfold, AssocList.keysList] at h' ⊢
-      simp at h'
-      simp only [Batteries.AssocList.find?_eq, Batteries.AssocList.toList]
-      rcases ident with ⟨ i1, i2 ⟩;
-      repeat (rw [List.find?_cons_of_neg]; rotate_left; simp; intros; subst_vars; solve_by_elim)
-      rfl
-  inputs_present := by sorry
-  outputs_present := by sorry
+-- instance {Tag T} : MatchInterface (rhsModule Tag T) (lhs_intModule Tag T) where
+--   input_types := by
+--     intro ident;
+--     by_cases h : (Batteries.AssocList.contains ↑ident (rhsModule Tag T).inputs)
+--     · have h' := AssocList.keysInMap h; fin_cases h' <;> rfl
+--     · have h' := AssocList.keysNotInMap h; dsimp [drunfold, AssocList.keysList] at h' ⊢
+--       simp at h'; let ⟨ ha, hb, hc ⟩ := h'; clear h'
+--       simp only [Batteries.AssocList.find?_eq, Batteries.AssocList.toList]
+--       rcases ident with ⟨ i1, i2 ⟩;
+--       repeat (rw [List.find?_cons_of_neg]; rotate_left; simp; intros; subst_vars; solve_by_elim)
+--       sorry
+--   output_types := by
+--     intro ident;
+--     by_cases h : (Batteries.AssocList.contains ↑ident (rhsModule Tag T).outputs)
+--     · have h' := AssocList.keysInMap h; fin_cases h' <;> rfl
+--     · have h' := AssocList.keysNotInMap h; dsimp [drunfold, AssocList.keysList] at h' ⊢
+--       simp at h'
+--       simp only [Batteries.AssocList.find?_eq, Batteries.AssocList.toList]
+--       rcases ident with ⟨ i1, i2 ⟩;
+--       repeat (rw [List.find?_cons_of_neg]; rotate_left; simp; intros; subst_vars; solve_by_elim)
+--       rfl
+--   inputs_present := by sorry
+--   outputs_present := by sorry
 
-instance {Tag T} : MatchInterface  (lhs_intModule Tag T) (lhsModule Tag T) where
-  input_types := by
-    intro ident;
-    by_cases h : (Batteries.AssocList.contains ↑ident (rhsModule Tag T).inputs)
-    · have h' := AssocList.keysInMap h; fin_cases h' <;> rfl
-    · have h' := AssocList.keysNotInMap h; dsimp [drunfold, AssocList.keysList] at h' ⊢
-      simp at h'; let ⟨ ha, hb, hc ⟩ := h'; clear h'
-      simp only [Batteries.AssocList.find?_eq, Batteries.AssocList.toList]
-      rcases ident with ⟨ i1, i2 ⟩;
-      repeat (rw [List.find?_cons_of_neg]; rotate_left; simp; intros; subst_vars; solve_by_elim)
-      sorry
-  output_types := by
-    intro ident;
-    by_cases h : (Batteries.AssocList.contains ↑ident (rhsModule Tag T).outputs)
-    · have h' := AssocList.keysInMap h; fin_cases h' <;> rfl
-    · have h' := AssocList.keysNotInMap h; dsimp [drunfold, AssocList.keysList] at h' ⊢
-      simp at h'
-      simp only [Batteries.AssocList.find?_eq, Batteries.AssocList.toList]
-      rcases ident with ⟨ i1, i2 ⟩;
-      repeat (rw [List.find?_cons_of_neg]; rotate_left; simp; intros; subst_vars; solve_by_elim)
-      rfl
-  inputs_present := by sorry
-  outputs_present := by sorry
+-- instance {Tag T} : MatchInterface  (lhs_intModule Tag T) (lhsModule Tag T) where
+--   input_types := by
+--     intro ident;
+--     by_cases h : (Batteries.AssocList.contains ↑ident (rhsModule Tag T).inputs)
+--     · have h' := AssocList.keysInMap h; fin_cases h' <;> rfl
+--     · have h' := AssocList.keysNotInMap h; dsimp [drunfold, AssocList.keysList] at h' ⊢
+--       simp at h'; let ⟨ ha, hb, hc ⟩ := h'; clear h'
+--       simp only [Batteries.AssocList.find?_eq, Batteries.AssocList.toList]
+--       rcases ident with ⟨ i1, i2 ⟩;
+--       repeat (rw [List.find?_cons_of_neg]; rotate_left; simp; intros; subst_vars; solve_by_elim)
+--       sorry
+--   output_types := by
+--     intro ident;
+--     by_cases h : (Batteries.AssocList.contains ↑ident (rhsModule Tag T).outputs)
+--     · have h' := AssocList.keysInMap h; fin_cases h' <;> rfl
+--     · have h' := AssocList.keysNotInMap h; dsimp [drunfold, AssocList.keysList] at h' ⊢
+--       simp at h'
+--       simp only [Batteries.AssocList.find?_eq, Batteries.AssocList.toList]
+--       rcases ident with ⟨ i1, i2 ⟩;
+--       repeat (rw [List.find?_cons_of_neg]; rotate_left; simp; intros; subst_vars; solve_by_elim)
+--       rfl
+--   inputs_present := by sorry
+--   outputs_present := by sorry
 
-#reduce rhsNames
-#reduce rhsModuleType
+-- #reduce rhsNames
+-- #reduce rhsModuleType
 
-#reduce lhsNames
-#reduce lhsModuleType
+-- #reduce lhsNames
+-- #reduce lhsModuleType
 
-#reduce lhs_intNames
-#reduce lhs_intModuleType
-
-
-
-def φ {Tag T} (state_rhs : rhsModuleType Tag T) (state_lhs : lhs_intModuleType Tag T) : Prop :=
-  let ⟨⟨x_branch_tag, x_branchC ⟩, x_fork, ⟨x_muxT, x_muxF, x_muxC⟩, ⟨x_join1_l, x_join1_r⟩, ⟨x_join2_l, x_join2_r⟩⟩ := state_rhs
-  let ⟨⟨y_join_tag, y_join_r⟩, ⟨y_muxT, y_muxF, y_muxC⟩⟩ := state_lhs
-  x_muxT.map Prod.snd ++ x_join1_r = List.map Prod.fst (List.filter (fun x => x.2 == true) y_join_r) ++ y_muxT ∧
-  x_muxF.map Prod.snd ++ x_join2_r = List.map Prod.fst (List.filter (fun x => x.2 == false) y_join_r) ++ y_muxF ∧
-  x_muxC ++ x_fork.2 = List.map Prod.snd y_join_r ++ y_muxC ∧
-  List.map Prod.fst (List.filter (fun x => x.2 == some true) (List.zipWithAll (fun a b => (a, b)) (y_join_tag) ((List.map Prod.snd y_join_r) ++ y_muxC ))) =
-  ((List.filterMap (fun | (some tag, some true) => some tag | _ => none) (List.zipWithAll (fun a b => (a, b)) (x_branch_tag) (x_branchC ++ x_fork.1)))) ++ x_join1_l ++ List.map Prod.fst x_muxT
-
-  -- List.map Prod.fst (List.filter (fun x => x.2 == false) (List.zipWithAll y_join_tag ((List.map Prod.snd y_join_r) ++ y_muxC ))) =
-  -- List.map Prod.fst (List.filter (fun x => x.2 == false) (List.zipWithAll x_branch_tag (x_branchC ++ x_fork.1))) ++ x_join2_l ++ List.map Prod.snd x_muxF ∧
-  -- y_muxC.head? = some true → y_muxT = [] ∧
-  -- y_muxC.head? = some false → y_muxF = []
-
-def φ' {Tag T} (state_rhs : rhsModuleType Tag T) (state_lhs : lhs_intModuleType Tag T) : Prop :=
-  let ⟨x_fork, ⟨x_muxT, x_muxF, x_muxC⟩, ⟨x_join1_l, x_join1_r⟩, ⟨x_join2_l, x_join2_r⟩⟩ := state_rhs
-  let ⟨⟨y_join_l, y_join_r⟩, ⟨y_muxT, y_muxF, y_muxC⟩⟩ := state_lhs
-  x_muxT.map Prod.snd ++ x_join1_r = List.map Prod.fst (List.filter (fun x => x.2 == true) y_join_r) ++ y_muxT ∧
-  x_muxF.map Prod.snd ++ x_join2_r = List.map Prod.fst (List.filter (fun x => x.2 == false) y_join_r) ++ y_muxF ∧
-  x_muxC = List.map Prod.snd y_join_r ++ y_muxC ∧
-  x_muxT.map Prod.fst ++ x_join1_l ++ x_fork  = y_join_l ∧
-  x_muxF.map Prod.fst ++ x_join2_l ++ x_fork   = y_join_l
-
-theorem add_element {α} (l l' l'' : List α) : l ++ l' = l ++ l'' -> l' = l'' := by
-  intro h
-  revert h
-  induction l
-  . simp
-  . rename_i a tail h1
-    simp
+-- #reduce lhs_intNames
+-- #reduce lhs_intModuleType
 
 
-theorem lhs_internal_correctness {Tag T}:
-  ∀ (x : rhsModuleType Tag T) (y : lhs_intModuleType Tag T), φ' x y -> ∃ y',
-    existSR [fun st st' =>
-    ∃ a b a_1 a_2 b_1 a_3,
-      ((false :: b_1 = st.2.2.2 ∧ a_1 = st.2.1 ∧ a_3 :: a_2 = st.2.2.1) ∧ st.1 = (a, b)) ∧
-          (st'.1.2 = b ++ [(a_3, false)] ∧ st'.1.1 = a) ∧ (a_1, a_2, b_1) = st'.2 ∨
-        ((true :: b_1 = st.2.2.2 ∧ a_3 :: a_1 = st.2.1 ∧ a_2 = st.2.2.1) ∧ st.1 = (a, b)) ∧
-          (st'.1.2 = b ++ [(a_3, true)] ∧ st'.1.1 = a) ∧ (a_1, a_2, b_1) = st'.2] y y'
-    ∧ φ x y' := by
-    intro x ⟨⟨y_join_l, y_join_r⟩, ⟨y_muxT, y_muxF, y_muxC⟩⟩ φ
-    revert y_join_r y_muxT y_muxF y_join_l x
-    induction y_muxC with
-    | nil =>
-      intros
-      constructor; constructor; constructor; constructor
-      . rename_i H; cases H
-        . simp_all only [beq_true, beq_false, List.append_nil, List.append_assoc]
-      . rename_i H; cases H
-        and_intros <;> simp_all
-    | cons currC y_muxC h =>
-      cases currC
-      . intro x y_join_l y_join_r y_muxT y_muxF φ
-        rcases y_muxF with _ | ⟨ output, y_muxF ⟩
-        . subst_vars
-          constructor; constructor
-          . constructor
-          . rcases φ with ⟨ φ₁, φ₂ ⟩
-            simp at φ₂
-            rcases φ₂ with ⟨ _, _, _, _ ⟩
-            simp at φ₁
-            constructor
-            . simp; subst_vars; assumption
-            . and_intros <;> subst_vars <;> try simp <;> try assumption
-              . rename_i hr
-                cases x
-                simp at hr
-                simp; assumption
-        . subst_vars
-          subst_vars
-          rcases x with ⟨x_fork, ⟨x_muxT, x_muxF, x_muxC⟩, ⟨x_join1_l, x_join1_r⟩, ⟨x_join2_l, x_join2_r⟩⟩
-          have : DataflowRewriter.MuxTaggedRewrite.φ' (x_fork, (x_muxT, x_muxF, x_muxC), (x_join1_l, x_join1_r), x_join2_l, x_join2_r)
-                ((y_join_l, y_join_r ++ [(output, false)]), y_muxT, y_muxF, y_muxC) := by
-            rcases φ with ⟨ φ₁, φ₂, φ₃, φ₄, φ₅ ⟩
-            unfold φ'; and_intros
-            all_goals simp_all
-          specialize h _ _ _ _ _ this
-          rcases h with ⟨ yl, h ⟩
-          apply Exists.intro ((_, _), (_, (_, _))); constructor
-          . apply existSR.step _ ((_, _), (_, (_, _))) _
-            . constructor
-            . constructor; constructor;constructor;
-              constructor; exists y_muxC, output
-              simp; and_intros
-              rfl; rfl; rfl; rfl; rfl; rfl; rfl; rfl; rfl
-            . apply h.left
-          . apply h.right
-      . intro x y_join_l y_join_r y_muxT y_muxF φ
-        rcases y_muxT with _ | ⟨ output, y_muxT ⟩
-        . subst_vars
-          constructor; constructor
-          . constructor
-          . rcases φ with ⟨ φ₁, φ₂ ⟩
-            simp at φ₂
-            rcases φ₂ with ⟨ _, _, _, _ ⟩
-            simp at φ₁
-            constructor
-            . simp; subst_vars; assumption
-            . and_intros <;> subst_vars <;> try simp <;> try assumption
-              . rename_i hr
-                cases x
-                simp at hr
-                simp; assumption
-        . subst_vars
-          subst_vars
-          rcases x with ⟨x_fork, ⟨x_muxT, x_muxF, x_muxC⟩, ⟨x_join1_l, x_join1_r⟩, ⟨x_join2_l, x_join2_r⟩⟩
-          have : DataflowRewriter.MuxTaggedRewrite.φ' (x_fork, (x_muxT, x_muxF, x_muxC), (x_join1_l, x_join1_r), x_join2_l, x_join2_r)
-                ((y_join_l, y_join_r ++ [(output, true)]), y_muxT, y_muxF, y_muxC) := by
-            rcases φ with ⟨ φ₁, φ₂, φ₃, φ₄, φ₅ ⟩
-            unfold φ'; and_intros
-            all_goals simp_all
-          specialize h _ _ _ _ _ this
-          rcases h with ⟨ yl, h ⟩
-          apply Exists.intro ((_, _), (_, (_, _))); constructor
-          . apply existSR.step _ ((_, _), (_, (_, _))) _
-            . constructor
-            . constructor; constructor;constructor;
-              constructor; exists y_muxC, output
-              simp; and_intros
-              rfl; rfl; rfl; rfl; rfl; rfl; rfl; rfl; rfl
-            . apply h.left
-          . apply h.right
+
+-- def φ {Tag T} (state_rhs : rhsModuleType Tag T) (state_lhs : lhs_intModuleType Tag T) : Prop :=
+--   let ⟨⟨x_branch_tag, x_branchC ⟩, x_fork, ⟨x_muxT, x_muxF, x_muxC⟩, ⟨x_join1_l, x_join1_r⟩, ⟨x_join2_l, x_join2_r⟩⟩ := state_rhs
+--   let ⟨⟨y_join_tag, y_join_r⟩, ⟨y_muxT, y_muxF, y_muxC⟩⟩ := state_lhs
+--   x_muxT.map Prod.snd ++ x_join1_r = List.map Prod.fst (List.filter (fun x => x.2 == true) y_join_r) ++ y_muxT ∧
+--   x_muxF.map Prod.snd ++ x_join2_r = List.map Prod.fst (List.filter (fun x => x.2 == false) y_join_r) ++ y_muxF ∧
+--   x_muxC ++ x_fork.2 = List.map Prod.snd y_join_r ++ y_muxC ∧
+--   List.map Prod.fst (List.filter (fun x => x.2 == some true) (List.zipWithAll (fun a b => (a, b)) (y_join_tag) ((List.map Prod.snd y_join_r) ++ y_muxC ))) =
+--   ((List.filterMap (fun | (some tag, some true) => some tag | _ => none) (List.zipWithAll (fun a b => (a, b)) (x_branch_tag) (x_branchC ++ x_fork.1)))) ++ x_join1_l ++ List.map Prod.fst x_muxT
+
+--   -- List.map Prod.fst (List.filter (fun x => x.2 == false) (List.zipWithAll y_join_tag ((List.map Prod.snd y_join_r) ++ y_muxC ))) =
+--   -- List.map Prod.fst (List.filter (fun x => x.2 == false) (List.zipWithAll x_branch_tag (x_branchC ++ x_fork.1))) ++ x_join2_l ++ List.map Prod.snd x_muxF ∧
+--   -- y_muxC.head? = some true → y_muxT = [] ∧
+--   -- y_muxC.head? = some false → y_muxF = []
+
+-- def φ' {Tag T} (state_rhs : rhsModuleType Tag T) (state_lhs : lhs_intModuleType Tag T) : Prop :=
+--   let ⟨x_fork, ⟨x_muxT, x_muxF, x_muxC⟩, ⟨x_join1_l, x_join1_r⟩, ⟨x_join2_l, x_join2_r⟩⟩ := state_rhs
+--   let ⟨⟨y_join_l, y_join_r⟩, ⟨y_muxT, y_muxF, y_muxC⟩⟩ := state_lhs
+--   x_muxT.map Prod.snd ++ x_join1_r = List.map Prod.fst (List.filter (fun x => x.2 == true) y_join_r) ++ y_muxT ∧
+--   x_muxF.map Prod.snd ++ x_join2_r = List.map Prod.fst (List.filter (fun x => x.2 == false) y_join_r) ++ y_muxF ∧
+--   x_muxC = List.map Prod.snd y_join_r ++ y_muxC ∧
+--   x_muxT.map Prod.fst ++ x_join1_l ++ x_fork  = y_join_l ∧
+--   x_muxF.map Prod.fst ++ x_join2_l ++ x_fork   = y_join_l
+
+-- theorem add_element {α} (l l' l'' : List α) : l ++ l' = l ++ l'' -> l' = l'' := by
+--   intro h
+--   revert h
+--   induction l
+--   . simp
+--   . rename_i a tail h1
+--     simp
 
 
+-- theorem lhs_internal_correctness {Tag T}:
+--   ∀ (x : rhsModuleType Tag T) (y : lhs_intModuleType Tag T), φ' x y -> ∃ y',
+--     existSR [fun st st' =>
+--     ∃ a b a_1 a_2 b_1 a_3,
+--       ((false :: b_1 = st.2.2.2 ∧ a_1 = st.2.1 ∧ a_3 :: a_2 = st.2.2.1) ∧ st.1 = (a, b)) ∧
+--           (st'.1.2 = b ++ [(a_3, false)] ∧ st'.1.1 = a) ∧ (a_1, a_2, b_1) = st'.2 ∨
+--         ((true :: b_1 = st.2.2.2 ∧ a_3 :: a_1 = st.2.1 ∧ a_2 = st.2.2.1) ∧ st.1 = (a, b)) ∧
+--           (st'.1.2 = b ++ [(a_3, true)] ∧ st'.1.1 = a) ∧ (a_1, a_2, b_1) = st'.2] y y'
+--     ∧ φ x y' := by
+--     intro x ⟨⟨y_join_l, y_join_r⟩, ⟨y_muxT, y_muxF, y_muxC⟩⟩ φ
+--     revert y_join_r y_muxT y_muxF y_join_l x
+--     induction y_muxC with
+--     | nil =>
+--       intros
+--       constructor; constructor; constructor; constructor
+--       . rename_i H; cases H
+--         . simp_all only [beq_true, beq_false, List.append_nil, List.append_assoc]
+--       . rename_i H; cases H
+--         and_intros <;> simp_all
+--     | cons currC y_muxC h =>
+--       cases currC
+--       . intro x y_join_l y_join_r y_muxT y_muxF φ
+--         rcases y_muxF with _ | ⟨ output, y_muxF ⟩
+--         . subst_vars
+--           constructor; constructor
+--           . constructor
+--           . rcases φ with ⟨ φ₁, φ₂ ⟩
+--             simp at φ₂
+--             rcases φ₂ with ⟨ _, _, _, _ ⟩
+--             simp at φ₁
+--             constructor
+--             . simp; subst_vars; assumption
+--             . and_intros <;> subst_vars <;> try simp <;> try assumption
+--               . rename_i hr
+--                 cases x
+--                 simp at hr
+--                 simp; assumption
+--         . subst_vars
+--           subst_vars
+--           rcases x with ⟨x_fork, ⟨x_muxT, x_muxF, x_muxC⟩, ⟨x_join1_l, x_join1_r⟩, ⟨x_join2_l, x_join2_r⟩⟩
+--           have : DataflowRewriter.MuxTaggedRewrite.φ' (x_fork, (x_muxT, x_muxF, x_muxC), (x_join1_l, x_join1_r), x_join2_l, x_join2_r)
+--                 ((y_join_l, y_join_r ++ [(output, false)]), y_muxT, y_muxF, y_muxC) := by
+--             rcases φ with ⟨ φ₁, φ₂, φ₃, φ₄, φ₅ ⟩
+--             unfold φ'; and_intros
+--             all_goals simp_all
+--           specialize h _ _ _ _ _ this
+--           rcases h with ⟨ yl, h ⟩
+--           apply Exists.intro ((_, _), (_, (_, _))); constructor
+--           . apply existSR.step _ ((_, _), (_, (_, _))) _
+--             . constructor
+--             . constructor; constructor;constructor;
+--               constructor; exists y_muxC, output
+--               simp; and_intros
+--               rfl; rfl; rfl; rfl; rfl; rfl; rfl; rfl; rfl
+--             . apply h.left
+--           . apply h.right
+--       . intro x y_join_l y_join_r y_muxT y_muxF φ
+--         rcases y_muxT with _ | ⟨ output, y_muxT ⟩
+--         . subst_vars
+--           constructor; constructor
+--           . constructor
+--           . rcases φ with ⟨ φ₁, φ₂ ⟩
+--             simp at φ₂
+--             rcases φ₂ with ⟨ _, _, _, _ ⟩
+--             simp at φ₁
+--             constructor
+--             . simp; subst_vars; assumption
+--             . and_intros <;> subst_vars <;> try simp <;> try assumption
+--               . rename_i hr
+--                 cases x
+--                 simp at hr
+--                 simp; assumption
+--         . subst_vars
+--           subst_vars
+--           rcases x with ⟨x_fork, ⟨x_muxT, x_muxF, x_muxC⟩, ⟨x_join1_l, x_join1_r⟩, ⟨x_join2_l, x_join2_r⟩⟩
+--           have : DataflowRewriter.MuxTaggedRewrite.φ' (x_fork, (x_muxT, x_muxF, x_muxC), (x_join1_l, x_join1_r), x_join2_l, x_join2_r)
+--                 ((y_join_l, y_join_r ++ [(output, true)]), y_muxT, y_muxF, y_muxC) := by
+--             rcases φ with ⟨ φ₁, φ₂, φ₃, φ₄, φ₅ ⟩
+--             unfold φ'; and_intros
+--             all_goals simp_all
+--           specialize h _ _ _ _ _ this
+--           rcases h with ⟨ yl, h ⟩
+--           apply Exists.intro ((_, _), (_, (_, _))); constructor
+--           . apply existSR.step _ ((_, _), (_, (_, _))) _
+--             . constructor
+--             . constructor; constructor;constructor;
+--               constructor; exists y_muxC, output
+--               simp; and_intros
+--               rfl; rfl; rfl; rfl; rfl; rfl; rfl; rfl; rfl
+--             . apply h.left
+--           . apply h.right
 
 
 
@@ -311,237 +309,239 @@ theorem lhs_internal_correctness {Tag T}:
 
 
 
-@[reducible] def cast_first {β : Type _ → Type _} {a b : (Σ α, β α)} (h : a = b) : a.fst = b.fst := by
-  subst_vars; rfl
-
-theorem sigma_rw {S T : Type _} {m m' : Σ (y : Type _), S → y → T → Prop} {x : S} {y : T} {v : m.fst}
-        (h : m = m' := by reduce; rfl) :
-  m.snd x v y ↔ m'.snd x ((cast_first h).mp v) y := by
-  constructor <;> (intros; subst h; assumption)
-
-theorem sigma_rw_simp {S T : Type _} {m m' : Σ (y : Type _), S → y → T → Prop} {x : S} {y : T} {v : m.fst}
-        (h : m = m' := by simp [drunfold,drcompute,seval]; rfl) :
-  m.snd x v y ↔ m'.snd x ((cast_first h).mp v) y := by
-  constructor <;> (intros; subst h; assumption)
-
-set_option maxHeartbeats 0
 
 
-theorem φ_indistinguishable {Tag T} :
-  ∀ x y, φ x y → Module.indistinguishable (rhsModule Tag T) (lhs_intModule Tag T) x y := by
-  unfold φ; intro ⟨x_fork, ⟨x_muxT, x_muxF, x_muxC⟩, ⟨x_join1_l, x_join1_r⟩, ⟨x_join2_l, x_join2_r⟩⟩ ⟨⟨y_join_l, y_join_r⟩, ⟨y_muxT, y_muxF, y_muxC⟩⟩ H
-  dsimp at *
-  constructor <;> intro ident new_i v Hcontains Hsem
-  . have Hkeys := AssocList.keysInMap Hcontains; clear Hcontains
-    fin_cases Hkeys
-    . simp [drunfold,drcompute,seval] at Hsem ⊢
-      rw[sigma_rw_simp] at Hsem; simp at Hsem
-      --rcases y_join with ⟨y_join_l, y_join_r⟩
-      apply Exists.intro ((_, _), (_, (_, _)))
-      constructor; dsimp; and_intros
-      all_goals rfl
-    . simp [drunfold,drcompute,seval] at Hsem ⊢
-      rw[sigma_rw_simp] at Hsem; simp at Hsem
-      apply Exists.intro ((_, _), (_, (_, _)))
-      constructor; dsimp; and_intros
-      all_goals rfl
-    . simp [drunfold,drcompute,seval] at Hsem ⊢
-      rw[sigma_rw_simp] at Hsem; simp at Hsem
-      apply Exists.intro ((_, _), (_, (_, _)))
-      constructor; dsimp; and_intros
-      all_goals rfl
-    . simp [drunfold,drcompute,seval] at Hsem ⊢
-      rw[sigma_rw_simp] at Hsem; simp at Hsem
-      --rcases y_join with ⟨y_join_l, y_join_r⟩
-      apply Exists.intro ((_, _), (_, (_, _)))
-      constructor; dsimp; and_intros
-      all_goals rfl
-  · have Hkeys := AssocList.keysInMap Hcontains; clear Hcontains
-    rcases new_i with ⟨x_new_fork, ⟨x_new_muxT, x_new_muxF, x_new_muxC⟩, ⟨x_new_join1_l, x_new_join1_r⟩, ⟨x_new_join2_l, x_new_join2_r⟩⟩
-    fin_cases Hkeys
-    . simp [drunfold,drcompute,seval] at Hsem ⊢
-      rw[sigma_rw_simp] at Hsem; simp at Hsem
-      rcases H with ⟨ H₁, H₂, H₃, H₄, H₅, H₆, H₇ ⟩
-      rcases v with ⟨ vt, vv ⟩
-      rcases Hsem with ⟨ ⟨ ⟨hsemll₁, hsemll₂, hsemll₃⟩ | ⟨hsemll₁, hsemll₂, hsemll₃⟩, ⟨⟨hsemlrll, hsemlrlr⟩, ⟨hsemlrrl, hsemlrrr⟩⟩ ⟩, hsemr ⟩
-      <;> subst_vars
-      . rcases y_join_r with _ | ⟨y_joint_r_h, y_join_r_t⟩
-        . dsimp at *; subst_vars; simp at H₇
-        . rcases y_joint_r_h with ⟨y_joint_r_h_val, y_joint_r_h_bool⟩; dsimp at *; subst_vars
-          simp at H₁ H₅
-          symm at H₂
-          symm at H₁
-          have H₂' := H₂
-          have H₁' := H₁
-          simp at hsemll₁; rcases hsemll₁; subst_vars
-          simp at H₂; cases H₂; subst_vars
-          apply Exists.intro ((_, _), (_, (_, _)))
-          rw [sigma_rw_simp]; dsimp
-          refine ⟨⟨?_, ?_⟩, rfl⟩
-          · symm at H₅
-            simp[List.append]
-            rw [H₅]
-          · left; rfl
-      . rcases y_join_r with _ | ⟨y_joint_r_h, y_join_r_t⟩
-        . dsimp at *; subst_vars; simp at H₆
-        . rcases y_joint_r_h with ⟨y_joint_r_h_val, y_joint_r_h_bool⟩; dsimp at *; subst_vars
-          simp at H₁ H₅
-          symm at H₂
-          symm at H₁
-          have H₂' := H₂
-          have H₁' := H₁
-          simp at hsemll₁; rcases hsemll₁; subst_vars
-          simp at H₁; cases H₁; subst_vars
-          apply Exists.intro ((_, _), (_, (_, _)))
-          rw [sigma_rw_simp]; dsimp
-          refine ⟨⟨?_, ?_⟩, rfl⟩
-          · rfl
-          · right; rfl
+-- @[reducible] def cast_first {β : Type _ → Type _} {a b : (Σ α, β α)} (h : a = b) : a.fst = b.fst := by
+--   subst_vars; rfl
 
-theorem correct_threeway_merge'' {Tag T: Type _} [DecidableEq T]:
-  rhsModule Tag T ⊑_{φ} lhs_intModule Tag T := by
-  intro x y HPerm
-  constructor
-  . admit
-  -- . intro ident new_i v Hcontains Hsem
-  --   rcases HPerm with ⟨ h₁, h₂, h₃, h₄, h₅, h₆, h₇ ⟩
-  --   have Hkeys := AssocList.keysInMap Hcontains; clear Hcontains
-  --   fin_cases Hkeys
-  --   . simp [drunfold,drcompute,seval] at Hsem ⊢
-  --     rw[sigma_rw_simp] at Hsem; simp at Hsem
-  --     rcases new_i with ⟨x_new_fork, ⟨x_new_muxT, x_new_muxF, x_new_muxC⟩, ⟨x_new_join1_l, x_new_join1_r⟩, ⟨x_new_join2_l, x_new_join2_r⟩⟩
-  --     subst_vars
-  --     apply Exists.intro ((_, _), (_, (_, _)))
-  --     rw [sigma_rw_simp]; dsimp
-  --     constructor
-  --     .  (repeat constructor) <;> rfl
-  --     . constructor; constructor
-  --       . constructor
-  --       . simp at Hsem; rcases Hsem with ⟨ Hsem₁, Hsem₂⟩
-  --         rcases x with ⟨x_fork, ⟨x_muxT, x_muxF, x_muxC⟩, ⟨x_join1_l, x_join1_r⟩, ⟨x_join2_l, x_join2_r⟩⟩
-  --         simp at Hsem₂
-  --         rcases Hsem₂ with ⟨ ⟨ _, _, _ ⟩ , ⟨ _, _ ⟩, _, _ ⟩
-  --         constructor
-  --         . simp
-  --           subst_vars
-  --           simp at *; assumption
-  --         . and_intros <;> (try subst_vars) <;> (try simp[*]) <;> (try assumption)
-  --           . simp_all only [beq_true, beq_false, List.append_assoc]
-  --             rw[← h₄]; simp
-  --           . simp_all only [beq_true, beq_false, List.append_assoc]
-  --             rw[← h₅]; simp
-  --   . simp [drunfold,drcompute,seval] at Hsem ⊢
-  --     rw[sigma_rw_simp] at Hsem; simp at Hsem
-  --     rcases new_i with ⟨x_new_fork, ⟨x_new_muxT, x_new_muxF, x_new_muxC⟩, ⟨x_new_join1_l, x_new_join1_r⟩, ⟨x_new_join2_l, x_new_join2_r⟩⟩
-  --     rcases y with ⟨⟨y_join_l, y_join_r⟩, ⟨y_muxT, y_muxF, y_muxC⟩⟩
-  --     subst_vars
-  --     apply Exists.intro ((_, _), (_, (_, _)))
-  --     rw [sigma_rw_simp]; dsimp
-  --     constructor
-  --     . (repeat constructor) <;> rfl
-  --     . apply lhs_internal_correctness
-  --       simp at Hsem; rcases Hsem with ⟨ Hsem₁, Hsem₂⟩
-  --       rcases x with ⟨x_fork, ⟨x_muxT, x_muxF, x_muxC⟩, ⟨x_join1_l, x_join1_r⟩, ⟨x_join2_l, x_join2_r⟩⟩
-  --       simp at Hsem₂
-  --       simp at Hsem₁
-  --       rcases Hsem₁ with ⟨ ⟨ _, _, _ ⟩ , ⟨ _, _ ⟩, _, _ ⟩
-  --       constructor <;> subst_vars <;> simp_all
-  --   . simp [drunfold,drcompute,seval] at Hsem ⊢
-  --     rw[sigma_rw_simp] at Hsem; simp at Hsem
-  --     rcases new_i with ⟨x_new_fork, ⟨x_new_muxT, x_new_muxF, x_new_muxC⟩, ⟨x_new_join1_l, x_new_join1_r⟩, ⟨x_new_join2_l, x_new_join2_r⟩⟩
-  --     rcases y with ⟨⟨y_join_l, y_join_r⟩, ⟨y_muxT, y_muxF, y_muxC⟩⟩
-  --     subst_vars
-  --     apply Exists.intro ((_, _), (_, (_, _)))
-  --     rw [sigma_rw_simp]; dsimp
-  --     constructor
-  --     . (repeat constructor) <;> rfl
-  --     . apply lhs_internal_correctness
-  --       simp at Hsem; rcases Hsem with ⟨ Hsem₁, Hsem₂⟩
-  --       rcases x with ⟨x_fork, ⟨x_muxT, x_muxF, x_muxC⟩, ⟨x_join1_l, x_join1_r⟩, ⟨x_join2_l, x_join2_r⟩⟩
-  --       simp at Hsem₂
-  --       simp at Hsem₁
-  --       rcases Hsem₁ with ⟨ ⟨ _, _, _ ⟩ , ⟨ _, _ ⟩, _, _ ⟩
-  --       subst_vars
-  --       constructor <;> simp_all
-  --       . rw[ ← List.append_assoc]
-  --         rw[ ← List.append_assoc]
-  --         simp_rw[← h₁]
-  --   . simp [drunfold,drcompute,seval] at Hsem ⊢
-  --     rw[sigma_rw_simp] at Hsem; simp at Hsem
-  --     rcases new_i with ⟨x_new_fork, ⟨x_new_muxT, x_new_muxF, x_new_muxC⟩, ⟨x_new_join1_l, x_new_join1_r⟩, ⟨x_new_join2_l, x_new_join2_r⟩⟩
-  --     rcases y with ⟨⟨y_join_l, y_join_r⟩, ⟨y_muxT, y_muxF, y_muxC⟩⟩
-  --     subst_vars
-  --     apply Exists.intro ((_, _), (_, (_, _)))
-  --     rw [sigma_rw_simp]; dsimp
-  --     constructor
-  --     . (repeat constructor) <;> rfl
-  --     . apply lhs_internal_correctness
-  --       simp at Hsem; rcases Hsem with ⟨ Hsem₁, Hsem₂⟩
-  --       rcases x with ⟨x_fork, ⟨x_muxT, x_muxF, x_muxC⟩, ⟨x_join1_l, x_join1_r⟩, ⟨x_join2_l, x_join2_r⟩⟩
-  --       simp at Hsem₂
-  --       simp at Hsem₁
-  --       rcases Hsem₁ with ⟨ ⟨ _, _, _ ⟩ , ⟨ _, _ ⟩, _, _ ⟩
-  --       subst_vars
-  --       constructor <;> simp_all
-  --       . rw[ ← List.append_assoc]
-  --         rw[ ← List.append_assoc]
-  --         simp_rw[← h₂]
-  . intro ident new_i v Hcontains Hsem
-    rcases HPerm with ⟨ h₁, h₂, h₃, h₄, h₅, h₆, h₇ ⟩
-    have Hkeys := AssocList.keysInMap Hcontains; clear Hcontains
-    fin_cases Hkeys
-    . simp [drunfold,drcompute,seval] at Hsem ⊢
-      rw[sigma_rw_simp] at Hsem; simp at Hsem
-      rcases new_i with ⟨x_new_fork, ⟨x_new_muxT, x_new_muxF, x_new_muxC⟩, ⟨x_new_join1_l, x_new_join1_r⟩, ⟨x_new_join2_l, x_new_join2_r⟩⟩
-      rcases x with ⟨x_fork, ⟨x_muxT, x_muxF, x_muxC⟩, ⟨x_join1_l, x_join1_r⟩, ⟨x_join2_l, x_join2_r⟩⟩
-      rcases y with ⟨⟨y_join_l, y_join_r⟩, ⟨y_muxT, y_muxF, y_muxC⟩⟩
-      subst_vars
-      rcases v with ⟨ouput_tag,ouput⟩
-      simp at Hsem
-      rcases Hsem with ⟨⟨⟨ H₁, H₂,H₃ ⟩ | ⟨H₄, H₅, H₆⟩⟩,  H₁₁⟩ <;> rename_i Hsem <;> rcases Hsem with ⟨ ⟨ H₇, H₈ ⟩, H₉, H₁₀⟩
-      <;> subst_vars <;> simp_all
-      . rw[List.cons_eq_append] at h₂
-        rcases h₂ with ⟨p₁, p₂, p₃ ⟩ | ⟨rest, p₂, p₃ ⟩
-        . simp at p₁
-          rcases y_join_r with _ | ⟨y_joint_r_h, y_join_r_t⟩
-          . simp at H₁; rw[← H₁] at h₇; simp at h₇
-          . simp at p₁
-            rcases y_joint_r_h with ⟨ a, b ⟩
-            specialize p₁ a; cases p₁
-            simp at H₁; rcases H₁ with ⟨ k, j ⟩
-            subst k; simp_all
-        . rcases y_join_r with _ | ⟨y_joint_r_h, y_join_r_t⟩
-          . simp_all
-          . apply Exists.intro ((_, _), (_, (_, _)))
-            rw [sigma_rw_simp]; dsimp
-            constructor
-            . (repeat constructor) <;> (try rfl)
-              . rw[← h₅]
-              . left
-                simp_all
-                constructor
-                . cases y_joint_r_h; simp at p₂; simp at H₁; simp_all
-                . rfl
-            . constructor; constructor
-              . constructor
-              . unfold φ; and_intros
-                . simp
-                  subst_vars
-                  cases y_joint_r_h
-                  simp_all
-                . cases y_joint_r_h; simp_all
-                . cases y_joint_r_h; simp_all
-                . rcases y_joint_r_h with ⟨ y_join_value, y_joint_condiction ⟩
-                  simp_all
-                  rcases p₂ with ⟨ p₂, p₂' ⟩
-                  rcases H₁ with ⟨ H₁, H₁'⟩
+-- theorem sigma_rw {S T : Type _} {m m' : Σ (y : Type _), S → y → T → Prop} {x : S} {y : T} {v : m.fst}
+--         (h : m = m' := by reduce; rfl) :
+--   m.snd x v y ↔ m'.snd x ((cast_first h).mp v) y := by
+--   constructor <;> (intros; subst h; assumption)
 
-                  rw[List.cons_eq_append] at h₅
-                  rcases h₅ with ⟨p₁, p₂, p₃ ⟩ | ⟨rest, p₂, p₃ ⟩
+-- theorem sigma_rw_simp {S T : Type _} {m m' : Σ (y : Type _), S → y → T → Prop} {x : S} {y : T} {v : m.fst}
+--         (h : m = m' := by simp [drunfold,drcompute,seval]; rfl) :
+--   m.snd x v y ↔ m'.snd x ((cast_first h).mp v) y := by
+--   constructor <;> (intros; subst h; assumption)
+
+-- set_option maxHeartbeats 0
 
 
-                  rw[← h₅]
-                  simp
+-- theorem φ_indistinguishable {Tag T} :
+--   ∀ x y, φ x y → Module.indistinguishable (rhsModule Tag T) (lhs_intModule Tag T) x y := by
+--   unfold φ; intro ⟨x_fork, ⟨x_muxT, x_muxF, x_muxC⟩, ⟨x_join1_l, x_join1_r⟩, ⟨x_join2_l, x_join2_r⟩⟩ ⟨⟨y_join_l, y_join_r⟩, ⟨y_muxT, y_muxF, y_muxC⟩⟩ H
+--   dsimp at *
+--   constructor <;> intro ident new_i v Hcontains Hsem
+--   . have Hkeys := AssocList.keysInMap Hcontains; clear Hcontains
+--     fin_cases Hkeys
+--     . simp [drunfold,drcompute,seval] at Hsem ⊢
+--       rw[sigma_rw_simp] at Hsem; simp at Hsem
+--       --rcases y_join with ⟨y_join_l, y_join_r⟩
+--       apply Exists.intro ((_, _), (_, (_, _)))
+--       constructor; dsimp; and_intros
+--       all_goals rfl
+--     . simp [drunfold,drcompute,seval] at Hsem ⊢
+--       rw[sigma_rw_simp] at Hsem; simp at Hsem
+--       apply Exists.intro ((_, _), (_, (_, _)))
+--       constructor; dsimp; and_intros
+--       all_goals rfl
+--     . simp [drunfold,drcompute,seval] at Hsem ⊢
+--       rw[sigma_rw_simp] at Hsem; simp at Hsem
+--       apply Exists.intro ((_, _), (_, (_, _)))
+--       constructor; dsimp; and_intros
+--       all_goals rfl
+--     . simp [drunfold,drcompute,seval] at Hsem ⊢
+--       rw[sigma_rw_simp] at Hsem; simp at Hsem
+--       --rcases y_join with ⟨y_join_l, y_join_r⟩
+--       apply Exists.intro ((_, _), (_, (_, _)))
+--       constructor; dsimp; and_intros
+--       all_goals rfl
+--   · have Hkeys := AssocList.keysInMap Hcontains; clear Hcontains
+--     rcases new_i with ⟨x_new_fork, ⟨x_new_muxT, x_new_muxF, x_new_muxC⟩, ⟨x_new_join1_l, x_new_join1_r⟩, ⟨x_new_join2_l, x_new_join2_r⟩⟩
+--     fin_cases Hkeys
+--     . simp [drunfold,drcompute,seval] at Hsem ⊢
+--       rw[sigma_rw_simp] at Hsem; simp at Hsem
+--       rcases H with ⟨ H₁, H₂, H₃, H₄, H₅, H₆, H₇ ⟩
+--       rcases v with ⟨ vt, vv ⟩
+--       rcases Hsem with ⟨ ⟨ ⟨hsemll₁, hsemll₂, hsemll₃⟩ | ⟨hsemll₁, hsemll₂, hsemll₃⟩, ⟨⟨hsemlrll, hsemlrlr⟩, ⟨hsemlrrl, hsemlrrr⟩⟩ ⟩, hsemr ⟩
+--       <;> subst_vars
+--       . rcases y_join_r with _ | ⟨y_joint_r_h, y_join_r_t⟩
+--         . dsimp at *; subst_vars; simp at H₇
+--         . rcases y_joint_r_h with ⟨y_joint_r_h_val, y_joint_r_h_bool⟩; dsimp at *; subst_vars
+--           simp at H₁ H₅
+--           symm at H₂
+--           symm at H₁
+--           have H₂' := H₂
+--           have H₁' := H₁
+--           simp at hsemll₁; rcases hsemll₁; subst_vars
+--           simp at H₂; cases H₂; subst_vars
+--           apply Exists.intro ((_, _), (_, (_, _)))
+--           rw [sigma_rw_simp]; dsimp
+--           refine ⟨⟨?_, ?_⟩, rfl⟩
+--           · symm at H₅
+--             simp[List.append]
+--             rw [H₅]
+--           · left; rfl
+--       . rcases y_join_r with _ | ⟨y_joint_r_h, y_join_r_t⟩
+--         . dsimp at *; subst_vars; simp at H₆
+--         . rcases y_joint_r_h with ⟨y_joint_r_h_val, y_joint_r_h_bool⟩; dsimp at *; subst_vars
+--           simp at H₁ H₅
+--           symm at H₂
+--           symm at H₁
+--           have H₂' := H₂
+--           have H₁' := H₁
+--           simp at hsemll₁; rcases hsemll₁; subst_vars
+--           simp at H₁; cases H₁; subst_vars
+--           apply Exists.intro ((_, _), (_, (_, _)))
+--           rw [sigma_rw_simp]; dsimp
+--           refine ⟨⟨?_, ?_⟩, rfl⟩
+--           · rfl
+--           · right; rfl
+
+-- theorem correct_threeway_merge'' {Tag T: Type _} [DecidableEq T]:
+--   rhsModule Tag T ⊑_{φ} lhs_intModule Tag T := by
+--   intro x y HPerm
+--   constructor
+--   . admit
+--   -- . intro ident new_i v Hcontains Hsem
+--   --   rcases HPerm with ⟨ h₁, h₂, h₃, h₄, h₅, h₆, h₇ ⟩
+--   --   have Hkeys := AssocList.keysInMap Hcontains; clear Hcontains
+--   --   fin_cases Hkeys
+--   --   . simp [drunfold,drcompute,seval] at Hsem ⊢
+--   --     rw[sigma_rw_simp] at Hsem; simp at Hsem
+--   --     rcases new_i with ⟨x_new_fork, ⟨x_new_muxT, x_new_muxF, x_new_muxC⟩, ⟨x_new_join1_l, x_new_join1_r⟩, ⟨x_new_join2_l, x_new_join2_r⟩⟩
+--   --     subst_vars
+--   --     apply Exists.intro ((_, _), (_, (_, _)))
+--   --     rw [sigma_rw_simp]; dsimp
+--   --     constructor
+--   --     .  (repeat constructor) <;> rfl
+--   --     . constructor; constructor
+--   --       . constructor
+--   --       . simp at Hsem; rcases Hsem with ⟨ Hsem₁, Hsem₂⟩
+--   --         rcases x with ⟨x_fork, ⟨x_muxT, x_muxF, x_muxC⟩, ⟨x_join1_l, x_join1_r⟩, ⟨x_join2_l, x_join2_r⟩⟩
+--   --         simp at Hsem₂
+--   --         rcases Hsem₂ with ⟨ ⟨ _, _, _ ⟩ , ⟨ _, _ ⟩, _, _ ⟩
+--   --         constructor
+--   --         . simp
+--   --           subst_vars
+--   --           simp at *; assumption
+--   --         . and_intros <;> (try subst_vars) <;> (try simp[*]) <;> (try assumption)
+--   --           . simp_all only [beq_true, beq_false, List.append_assoc]
+--   --             rw[← h₄]; simp
+--   --           . simp_all only [beq_true, beq_false, List.append_assoc]
+--   --             rw[← h₅]; simp
+--   --   . simp [drunfold,drcompute,seval] at Hsem ⊢
+--   --     rw[sigma_rw_simp] at Hsem; simp at Hsem
+--   --     rcases new_i with ⟨x_new_fork, ⟨x_new_muxT, x_new_muxF, x_new_muxC⟩, ⟨x_new_join1_l, x_new_join1_r⟩, ⟨x_new_join2_l, x_new_join2_r⟩⟩
+--   --     rcases y with ⟨⟨y_join_l, y_join_r⟩, ⟨y_muxT, y_muxF, y_muxC⟩⟩
+--   --     subst_vars
+--   --     apply Exists.intro ((_, _), (_, (_, _)))
+--   --     rw [sigma_rw_simp]; dsimp
+--   --     constructor
+--   --     . (repeat constructor) <;> rfl
+--   --     . apply lhs_internal_correctness
+--   --       simp at Hsem; rcases Hsem with ⟨ Hsem₁, Hsem₂⟩
+--   --       rcases x with ⟨x_fork, ⟨x_muxT, x_muxF, x_muxC⟩, ⟨x_join1_l, x_join1_r⟩, ⟨x_join2_l, x_join2_r⟩⟩
+--   --       simp at Hsem₂
+--   --       simp at Hsem₁
+--   --       rcases Hsem₁ with ⟨ ⟨ _, _, _ ⟩ , ⟨ _, _ ⟩, _, _ ⟩
+--   --       constructor <;> subst_vars <;> simp_all
+--   --   . simp [drunfold,drcompute,seval] at Hsem ⊢
+--   --     rw[sigma_rw_simp] at Hsem; simp at Hsem
+--   --     rcases new_i with ⟨x_new_fork, ⟨x_new_muxT, x_new_muxF, x_new_muxC⟩, ⟨x_new_join1_l, x_new_join1_r⟩, ⟨x_new_join2_l, x_new_join2_r⟩⟩
+--   --     rcases y with ⟨⟨y_join_l, y_join_r⟩, ⟨y_muxT, y_muxF, y_muxC⟩⟩
+--   --     subst_vars
+--   --     apply Exists.intro ((_, _), (_, (_, _)))
+--   --     rw [sigma_rw_simp]; dsimp
+--   --     constructor
+--   --     . (repeat constructor) <;> rfl
+--   --     . apply lhs_internal_correctness
+--   --       simp at Hsem; rcases Hsem with ⟨ Hsem₁, Hsem₂⟩
+--   --       rcases x with ⟨x_fork, ⟨x_muxT, x_muxF, x_muxC⟩, ⟨x_join1_l, x_join1_r⟩, ⟨x_join2_l, x_join2_r⟩⟩
+--   --       simp at Hsem₂
+--   --       simp at Hsem₁
+--   --       rcases Hsem₁ with ⟨ ⟨ _, _, _ ⟩ , ⟨ _, _ ⟩, _, _ ⟩
+--   --       subst_vars
+--   --       constructor <;> simp_all
+--   --       . rw[ ← List.append_assoc]
+--   --         rw[ ← List.append_assoc]
+--   --         simp_rw[← h₁]
+--   --   . simp [drunfold,drcompute,seval] at Hsem ⊢
+--   --     rw[sigma_rw_simp] at Hsem; simp at Hsem
+--   --     rcases new_i with ⟨x_new_fork, ⟨x_new_muxT, x_new_muxF, x_new_muxC⟩, ⟨x_new_join1_l, x_new_join1_r⟩, ⟨x_new_join2_l, x_new_join2_r⟩⟩
+--   --     rcases y with ⟨⟨y_join_l, y_join_r⟩, ⟨y_muxT, y_muxF, y_muxC⟩⟩
+--   --     subst_vars
+--   --     apply Exists.intro ((_, _), (_, (_, _)))
+--   --     rw [sigma_rw_simp]; dsimp
+--   --     constructor
+--   --     . (repeat constructor) <;> rfl
+--   --     . apply lhs_internal_correctness
+--   --       simp at Hsem; rcases Hsem with ⟨ Hsem₁, Hsem₂⟩
+--   --       rcases x with ⟨x_fork, ⟨x_muxT, x_muxF, x_muxC⟩, ⟨x_join1_l, x_join1_r⟩, ⟨x_join2_l, x_join2_r⟩⟩
+--   --       simp at Hsem₂
+--   --       simp at Hsem₁
+--   --       rcases Hsem₁ with ⟨ ⟨ _, _, _ ⟩ , ⟨ _, _ ⟩, _, _ ⟩
+--   --       subst_vars
+--   --       constructor <;> simp_all
+--   --       . rw[ ← List.append_assoc]
+--   --         rw[ ← List.append_assoc]
+--   --         simp_rw[← h₂]
+--   . intro ident new_i v Hcontains Hsem
+--     rcases HPerm with ⟨ h₁, h₂, h₃, h₄, h₅, h₆, h₇ ⟩
+--     have Hkeys := AssocList.keysInMap Hcontains; clear Hcontains
+--     fin_cases Hkeys
+--     . simp [drunfold,drcompute,seval] at Hsem ⊢
+--       rw[sigma_rw_simp] at Hsem; simp at Hsem
+--       rcases new_i with ⟨x_new_fork, ⟨x_new_muxT, x_new_muxF, x_new_muxC⟩, ⟨x_new_join1_l, x_new_join1_r⟩, ⟨x_new_join2_l, x_new_join2_r⟩⟩
+--       rcases x with ⟨x_fork, ⟨x_muxT, x_muxF, x_muxC⟩, ⟨x_join1_l, x_join1_r⟩, ⟨x_join2_l, x_join2_r⟩⟩
+--       rcases y with ⟨⟨y_join_l, y_join_r⟩, ⟨y_muxT, y_muxF, y_muxC⟩⟩
+--       subst_vars
+--       rcases v with ⟨ouput_tag,ouput⟩
+--       simp at Hsem
+--       rcases Hsem with ⟨⟨⟨ H₁, H₂,H₃ ⟩ | ⟨H₄, H₅, H₆⟩⟩,  H₁₁⟩ <;> rename_i Hsem <;> rcases Hsem with ⟨ ⟨ H₇, H₈ ⟩, H₉, H₁₀⟩
+--       <;> subst_vars <;> simp_all
+--       . rw[List.cons_eq_append] at h₂
+--         rcases h₂ with ⟨p₁, p₂, p₃ ⟩ | ⟨rest, p₂, p₃ ⟩
+--         . simp at p₁
+--           rcases y_join_r with _ | ⟨y_joint_r_h, y_join_r_t⟩
+--           . simp at H₁; rw[← H₁] at h₇; simp at h₇
+--           . simp at p₁
+--             rcases y_joint_r_h with ⟨ a, b ⟩
+--             specialize p₁ a; cases p₁
+--             simp at H₁; rcases H₁ with ⟨ k, j ⟩
+--             subst k; simp_all
+--         . rcases y_join_r with _ | ⟨y_joint_r_h, y_join_r_t⟩
+--           . simp_all
+--           . apply Exists.intro ((_, _), (_, (_, _)))
+--             rw [sigma_rw_simp]; dsimp
+--             constructor
+--             . (repeat constructor) <;> (try rfl)
+--               . rw[← h₅]
+--               . left
+--                 simp_all
+--                 constructor
+--                 . cases y_joint_r_h; simp at p₂; simp at H₁; simp_all
+--                 . rfl
+--             . constructor; constructor
+--               . constructor
+--               . unfold φ; and_intros
+--                 . simp
+--                   subst_vars
+--                   cases y_joint_r_h
+--                   simp_all
+--                 . cases y_joint_r_h; simp_all
+--                 . cases y_joint_r_h; simp_all
+--                 . rcases y_joint_r_h with ⟨ y_join_value, y_joint_condiction ⟩
+--                   simp_all
+--                   rcases p₂ with ⟨ p₂, p₂' ⟩
+--                   rcases H₁ with ⟨ H₁, H₁'⟩
+
+--                   rw[List.cons_eq_append] at h₅
+--                   rcases h₅ with ⟨p₁, p₂, p₃ ⟩ | ⟨rest, p₂, p₃ ⟩
+
+
+--                   rw[← h₅]
+--                   simp
 
 
 
