DataflowRewriter/Rewrites/MuxToTaggedMux.lean
@@ -7,7 +7,7 @@ Authors: Yann Herklotz
 import DataflowRewriter.Rewriter
 import DataflowRewriter.ExprHighElaborator
 
-namespace DataflowRewriter.BranchMuxToMerge
+namespace DataflowRewriter.MuxToTaggedMux
 
 -- The following namespace just shows two alternative definitions of the matcher
 -- and the abstraction matcher that use the domination algorithm instead of
@@ -228,4 +228,4 @@ def lhs' : ExprHigh String := [graph|
 
 end TEST
 
-end DataflowRewriter.BranchMuxToMerge
+end DataflowRewriter.MuxToTaggedMux
